4章終わり

Prog_Prove_3_5.thy
@@ -133,6 +133,126 @@ lemma ST: "S w \<Longrightarrow> T w"
 corollary SeqT: "S w \<longleftrightarrow> T w"
   using ST TS by blast
 
-(*---------------- Exercise 4.6----------------*)
+(* Exercise 4.6 *)
+
+type_synonym vname = string
+datatype aexp = N int | V vname | Plus aexp aexp
+type_synonym val = int
+type_synonym state = "vname \<Rightarrow> val" 
+
+fun aval :: "aexp \<Rightarrow> state \<Rightarrow> val" where
+"aval (N n) s = n" |
+"aval (V x) s = s x" |
+"aval (Plus x y) s = aval x s + aval y s" 
+
+inductive aval_rel2 :: "aexp \<Rightarrow> state \<Rightarrow> val \<Rightarrow> bool" where
+rel_nat: "aval_rel2 (N n) s n" |
+rel_var: "s x = n \<Longrightarrow> aval_rel2 (V x) s n" |
+rel_plus: "(aval_rel2 x s n1) \<Longrightarrow>  (aval_rel2 y s n2) \<Longrightarrow> aval_rel2 (Plus x y) s (n1 + n2)"
+
+lemma aval_rel_to_aval: "aval_rel2 x s v \<Longrightarrow> (aval x s = v)"
+  apply(induction rule: aval_rel2.induct)
+  apply(auto)
+  done
+
+lemma aval_to_aval_rel: "(aval x s = v) \<Longrightarrow> aval_rel2 x s v"
+  apply(induction x arbitrary: v)
+(*    apply (simp add: rel_nat)
+   apply (simp add: rel_var)
+ apply (simp add: rel_plus) *)
+  apply(auto intro: rel_nat rel_var rel_plus)
+  done
+
+lemma "(aval_rel2 x s v) \<longleftrightarrow> (aval x s = v)"
+  apply(auto simp add: aval_rel_to_aval)
+  apply(auto simp add: aval_to_aval_rel)
+  done
+
+(* Exercise 4.7. *)
+
+datatype instr = LOADI val | LOAD vname | ADD
+
+type_synonym stack = "val list"
+
+fun exec1 :: "instr \<Rightarrow> state \<Rightarrow> stack \<Rightarrow> stack" where
+"exec1 (LOADI n) _ stk = n # stk" |
+"exec1 (LOAD x) s stk = s(x) # stk" |
+"exec1 ADD _ (j # i # stk) = (i + j) # stk"
+
+fun exec :: "instr list \<Rightarrow> state \<Rightarrow> stack \<Rightarrow> stack" where
+"exec [] _ stk = stk" |
+"exec (i#is) s stk = exec is s (exec1 i s stk)"
+
+lemma exec_division: "exec (is1 @ is2) s stk = exec is2 s (exec is1 s stk)"
+  apply(induction is1 arbitrary:stk)
+   apply(auto)
+  done
+
+lemma exec_append: "exec is\<^sub>1 s stk = stk' \<Longrightarrow> exec (is\<^sub>1 @ is\<^sub>2) s stk = exec is\<^sub>2 s stk'"
+apply(induction is\<^sub>1 arbitrary: stk)
+apply(auto)
+done
+
+fun comp:: "aexp \<Rightarrow> instr list" where
+"comp (N n) = [LOADI n]" |
+"comp (V x) = [LOAD x]" |
+"comp (Plus e1 e2) = comp e1 @ comp e2 @ [ADD]"
+
+lemma "exec (comp x) s stk = aval x s # stk"
+  apply(induction x arbitrary:stk)
+    apply(auto simp add: exec_division )
+  done
+
+(* the size of the execution become + 1 when LOADI or LOAD
+but when ADD which is compiled and become -1.
+*)
+inductive  ok :: "nat \<Rightarrow> instr list \<Rightarrow> nat \<Rightarrow> bool" where 
+ok_emp: "ok n [] n" |
+ok_LOADI: "ok n is n'  \<Longrightarrow> ok n (is @ [LOADI _]) (n' + 1)" |
+ok_LOAD: "ok n is n'  \<Longrightarrow> ok n (is @ [LOAD _]) (n' + 1)" |
+(* when n' = 0 or 1, n' -1 would be not nat*)
+ok_ADD: "ok n is (n' + 2)   \<Longrightarrow> ok n (is @ [ADD]) (n' + 1)"
+
+(*
+lemma "length (exec is s stk) = Suc (Suc n') \<Longrightarrow>
+       length (exec1 ADD s (exec is s stk)) = Suc n'"
+  by (smt Nitpick.size_list_simp(2) add_diff_cancel_left' exec1.elims instr.distinct(3) instr.distinct(5) list.sel(3) nat.distinct(1) null_rec(1) null_rec(2) plus_1_eq_Suc)
+*)
+
+
+lemma "\<lbrakk>ok n is n'; length stk = n \<rbrakk> \<Longrightarrow> length (exec is s stk) = n'"
+  apply(induction rule: ok.induct)
+    apply(auto simp add: exec_division)
+  by (smt exec1.elims instr.distinct(3) instr.distinct(5) length_Cons list.size(3) nat.distinct(1) nat.inject)
+
+
+ (* The followings are timed-out:
+  by (smt exec1.elims instr.distinct(3) instr.distinct(5) length_Cons list.size(3) nat.distinct(1) nat.inject)
+  by (smt Nitpick.size_list_simp(2) add_left_cancel exec1.elims instr.distinct(3) instr.distinct(5) length_Cons nat.distinct(1) plus_1_eq_Suc)
+*)
+
+(* the followings are copied and pasted from following github:
+https://github.com/cmr/ConcreteSemantics/blob/master/CS_Ch4.thy
+
+I couldn't understand what have done and how to know this proof.
+*)
+
+(* TODO: try again!*)
+lemma ok_append: "ok n (e2) n' \<Longrightarrow> ok n'' (e1) n \<Longrightarrow> ok n'' (e1 @ e2) n'"
+apply(induction rule: ok.induct)
+apply(simp)
+apply (metis append_assoc ok.simps)
+apply (metis append_assoc ok.simps)
+apply (metis append_assoc ok.simps)
+done
+
+
+lemma "ok n (comp x) (Suc n)"
+apply(induction x arbitrary: n)
+
+using ok_LOADI ok_emp apply fastforce
+using ok_LOAD ok_emp apply fastforce
+using ok_ADD ok_append apply fastforce
+  done
 
 end
